---
layout: post
title: A MathJax Excersize
subtitle: Proof of Cauchy-Schwarz in an L<sub>2</sub> inner product space.
gh-repo: daattali/beautiful-jekyll
gh-badge: [star, fork, follow]
tags: [test]
comments: true
---

Given two continuous function $f:[0,1] \xrightarrow{} \mathbb{R}$ and $g:[0,1]  \xrightarrow{} \mathbb{R}$, we define the L<sub>2</sub> inner product of _f_ and _g_, denoted by $\langle f,g\rangle$, by the formula

 $\int_{0}^{1} f(x)g(x)dx$. 
 
 We can quickly check that this is an inner product by showing it satisfies the linearity and symmetric properties.
 
 - Linearity
 
 $\langle \alpha f + \beta g, h\rangle = \int_0^1 (\alpha f(x) + \beta g(x)) h(x) dx = \int_0^1\alpha f(x)h(x) + \int_0^1 \beta g(x)h(x)$

$ = \alpha\langle f,h\rangle + \beta\langle g,h \rangle.$

- Symmetry

$\langle f,g\rangle =\int_0^1 f(x)g(x)dx = \int_0^1 g(x)f(x)dx= \langle g,f\rangle$

Now, since we know that this is an inner product, we already know that the Cauchy-Schwarz inequalioty applies, but sometimes it can be enlightening to build a proof in the context with which you are working. So, in this spirit, we aim to prove the Cauchy-Schwarz inequality which (in this context) is stated as follows: 

$\left\lvert \int_{0}^{1} f(x)g(x)dx \right\rvert \leq \sqrt{\int_{0}^{1} [f(x)]^2dx}\sqrt{\int_{0}^{1} [g(x)]^2dx}$

Before doing so, it is convenient to establish the idea of orthogonality.

#####Definition
Two functions _f_ and _g_ are said to be orthogonal if $\langle f, g \rangle = 0$. In this context, that is $\int_0^1 f(x)g(x)dx=0$, in our context. 

From here, we define $\lambda= \frac{\langle f,g \rangle}{\langle g,g\rangle}$ and $h= f-\lambda g$. It is not hard to show that _h_ is orthogonal to _g_. With these tools, the proof turns out to be rather simple. 


## Proof
**a**. If either _f_ or _g_ are identically 0 along the interval, equality clearly holds and both sides are 0. 
**b**. Now, under the assumption that neither _f_ nor _g_ are identically 0, we prove the theorem as follows. 

For any function _F_, we know that $0 \leq \int_0^1[F(x)]^2dx$. Now, using our function _h_ in place of _f_, we have that 

$ 0 \leq \int_0^1[f(x)-\lambda g(x)][f(x)-\lambda g(x)] dx= \int_0^1[f(x)-\lambda g(x)]f(x) dx + \int_0^1[f(x)-\lambda g(x)]g(x)dx $

Here, hopefully you can see that the last term is $\langle h,g \rangle$ which is 0 due to _h_ and _g_ being orthogonal by the definition of _h_. So, we reduce this to the equation 

$0 \leq \int_0^1[f(x)-\lambda g(x)]f(x) dx = \int_0^1[f(x)^2]dx -\lambda \int_0^1 f(x)g(x)dx$.

Now, since we have that 

$\lambda = \frac{\int_0^1 f(x)g(x)dx}{\int_0^1 g(x)g(x)dx}$

we can re-write the equation by multiplying by the denominator and moving the last term left. Then we get

$[\int_0^1 f(x)g(x)dx]^2 \leq [\int_0^1[f(x)^2]dx] [\int_0^1[g(x)^2]dx ]$

Finally, by taking the root of both sides we obtain 

$\left\lvert \int_{0}^{1} f(x)g(x)dx \right\rvert \leq \sqrt{\int_{0}^{1} [f(x)]^2dx}\sqrt{\int_{0}^{1} [g(x)]^2dx}$.
